Make call_k more flexible

SkLean/Candidates2.lean
@@ -1,27 +1,62 @@
 import SkLean.Ast2
+import SkLean.Typing2
+import SkLean.Sn2
 
-/-
-# Hierarchied SK Reducibility Candidates
+def is_candidate_for (e : Expr) (t : Expr) : Prop := valid_judgment e t ∧ e.valid_universes
 
--/
+namespace valid_judgment
 
-inductive is_candidate_n : ℕ → Expr → Expr → Prop
-  | stuck : (¬(∃ e', is_eval_once e e')) → is_candidate_n 0 e e
-  | succ  : is_eval_once e e'
-    → e_final.max_universe < e.max_universe
-    → is_candidate_n n e' e_final
-    → is_candidate_n n.succ e e_final
+lemma imp_is_candidate_for : valid_judgment e t → is_candidate_for e t := by
+  intro h_t
+  unfold is_candidate_for
+  induction h_t
+  constructor
+  apply valid_judgment.k
+  apply Expr.valid_universes.k
+  constructor
+  apply valid_judgment.s
+  apply Expr.valid_universes.s
+  constructor
+  apply valid_judgment.m
+  apply Expr.valid_universes.m
+  case call lhs rhs h_u h_t_lhs h_t_rhs ih₁ ih₂ =>
+    simp_all
+    constructor
+    apply valid_judgment.call
+    exact h_u
+    simp_all
+    simp_all
+    apply Expr.valid_universes.call
+    exact h_u
+    simp_all
+    simp_all
+
+end valid_judgment
 
 namespace is_candidate_for
 
-lemma imp_judgment : is_candidate_for e t → valid_judgment e t := by
-  intro h_r
-  induction h_r
-  case stuck t' h_step h =>
-    exact h
-  case step e' t' h_beq h_u =>
-    
+lemma imp_sn : is_candidate_for e t → sn e := fun ⟨h_t_lhs, h_t_rhs⟩ => by
+  induction h_t_lhs
+  apply sn.k
+  apply sn.s
+  apply sn.m
+  case call lhs rhs h_u h_t_lhs h_t_rhs h_candidate_lhs h_candidate_rhs ih =>
+    cases h_t_rhs
+    simp_all
+    apply valid_judgment.imp_is_candidate_for at h_t_lhs
+    apply valid_judgment.imp_is_candidate_for at h_t_rhs
+    simp_all
+    match h : SKM[(lhs rhs)] with
+      | SKM[(((K n) x) y)] =>
+        
+        sorry
     sorry
+
+lemma imp_judgment : is_candidate_for e t → valid_judgment e t :=
+  fun ⟨h_t_lh, _⟩ => h_t_lh
+
+lemma imp_valid_universes : is_candidate_for e t → e.valid_universes :=
+  fun ⟨_, h_t_rh⟩ => h_t_rh
 
 end is_candidate_for
 
